Instances/IsBool/Boolean.v
@@ -7,8 +7,8 @@ Require Import Types.Result.
 
 Definition ensure_bool (v : cvalue) : State bool :=
   fun st => match v with
-            | VBool b => returnR bool store b st
-            | _ => crashed _ _
+            | VBool b => returnR b st
+            | _ => crashed 
             end.
 
 Definition build_boolean (b : bool) : State cvalue :=
@@ -27,8 +27,8 @@ Definition eval_if {A} (b : bool) (st1 st2 : State A) : State A :=
 Instance boolean_type : IsBool State cvalue bool :=
 {
   ensure_bool := ensure_bool;
-  extract_bool := extract_boolean;
   build_bool := build_boolean;
+  extract_bool := fun b => returnM b;
   and_op := andbM;
   neg_op := negbM;
   if_op := eval_if;
