Instances/Store/ConcreteStore.v
@@ -6,13 +6,10 @@ Require Import Types.Result.
 Require Import Types.Stores.
 
 Definition store_get (x : string) : State cvalue := fun st =>
-  returnR cvalue store (st x) st.
+  returnR (st x) st.
 
 Definition store_put (x : string) (v : cvalue) : State unit := 
-  fun st => returnR unit store tt (t_update st x v).
-
-Check store_put.
-Check put.
+  fun st => returnR tt (t_update st x v).
 
 Instance store_concrete : Store State cvalue := {
   get := store_get;
