Instances/Except/ConcreteException.v
@@ -5,13 +5,13 @@ Require Import Types.Stores.
 
 Definition eval_catch {A} (st1 st2 : State A) : State A :=
   fun st => match (st1 st) with
-  | crashed _ _ => crashed _ _
-  | exception _ _ st' => (st2 st')
+  | crashed => crashed 
+  | exception st' => (st2 st')
   | x => x
   end.
 
 Definition fail {A : Type} : State A :=
-  fun st => exception A store st.
+  fun st => exception st.
 
 Instance except_concrete : Except State := {
   throw := fail;
