Instances/Preorder/Result.v
@@ -7,25 +7,24 @@ Section result_preorder.
 Context {A S: Type} `{PreorderedSet A, PreorderedSet S}.
 
 Inductive result_le : abstract_result A S -> abstract_result A S -> Prop :=
-  | result_le_crashed : forall r, result_le r (crashedA A S)
+  | result_le_crashed : forall r, result_le r (crashedA )
   | result_le_exception : forall s1 s2, 
-      preorder s1 s2 -> result_le (exceptionA A S s1) (exceptionA A S s2)
+      preorder s1 s2 -> result_le (exceptionA s1) (exceptionA s2)
   | result_le_return : forall a1 a2 s1 s2, 
       preorder a1 a2 -> 
       preorder s1 s2 ->
-      result_le (returnRA A S a1 s1) (returnRA A S a2 s2)
+      result_le (returnRA a1 s1) (returnRA a2 s2)
   | result_le_exception_or : forall a st1 st2, 
       preorder st1 st2 -> 
-      result_le (exceptionA A S st1) (exceptionOrReturn A S a st2)
+      result_le (exceptionA st1) (exceptionOrReturn a st2)
   | result_le_return_or : forall a1 a2 s1 s2,
       preorder s1 s2 ->
       preorder a1 a2 ->
-      result_le (returnRA A S a1 s1) (exceptionOrReturn A S a2 s2)
+      result_le (returnRA a1 s1) (exceptionOrReturn a2 s2)
   | result_le_or_or : forall a1 a2 s1 s2,
       preorder a1 a2 ->
       preorder s1 s2 ->
-      result_le (exceptionOrReturn A S a1 s1) (exceptionOrReturn A S a2 s2).
-
+      result_le (exceptionOrReturn a1 s1) (exceptionOrReturn a2 s2).
 
 Lemma result_le_refl :
   Reflexive result_le.
