Types/Result.v
@@ -9,11 +9,20 @@ Inductive result (A S : Type) : Type :=
   | returnR : A -> S -> result A S
   | crashed : result A S
   | exception : S -> result A S.
+
+Arguments returnR {_ _}.
+Arguments crashed {_ _}.
+Arguments exception {_ _}.
   
 Inductive abstract_result (A S : Type) :=
   | returnRA : A -> S -> abstract_result A S
   | crashedA : abstract_result A S
   | exceptionA : S -> abstract_result A S
   | exceptionOrReturn : A -> S -> abstract_result A S.
+
+Arguments returnRA {_ _}.
+Arguments crashedA {_ _}.
+Arguments exceptionA {_ _}.
+Arguments exceptionOrReturn {_ _}.
 
 
